Arithmetization/ISigmaOne/Metamath/Term/Basic.lean
@@ -143,23 +143,23 @@ open FormalizedTerm
 
 variable (L)
 
-def Language.IsSemiterm (n : V) : V → Prop := (construction L).Fixpoint ![n]
+def Language.Semiterm (n : V) : V → Prop := (construction L).Fixpoint ![n]
 
 def _root_.LO.FirstOrder.Arith.LDef.isSemitermDef (pL : LDef) : 𝚫₁-Semisentence 2 := (formula pL).fixpointDefΔ₁.rew (Rew.substs ![#1, #0])
 
-lemma isSemiterm_defined : 𝚫₁-Relation L.IsSemiterm via pL.isSemitermDef :=
+lemma isSemiterm_defined : 𝚫₁-Relation L.Semiterm via pL.isSemitermDef :=
   ⟨HSemiformula.ProperOn.rew (construction L).fixpoint_definedΔ₁.proper _,
    by intro v; simp [LDef.isSemitermDef, (construction L).eval_fixpointDefΔ₁]; rfl⟩
 
 @[simp] lemma eval_isSemitermDef (v) :
-    Semiformula.Evalbm V v pL.isSemitermDef.val ↔ L.IsSemiterm (v 0) (v 1) := (isSemiterm_defined L).df.iff v
+    Semiformula.Evalbm V v pL.isSemitermDef.val ↔ L.Semiterm (v 0) (v 1) := (isSemiterm_defined L).df.iff v
 
-instance isSemitermDef_definable : 𝚫₁-Relation (L.IsSemiterm) := Defined.to_definable _ (isSemiterm_defined L)
+instance isSemitermDef_definable : 𝚫₁-Relation (L.Semiterm) := Defined.to_definable _ (isSemiterm_defined L)
 
-@[simp, definability] instance isSemitermDef_definable' (Γ) : (Γ, m + 1)-Relation (L.IsSemiterm) :=
+@[simp, definability] instance isSemitermDef_definable' (Γ) : (Γ, m + 1)-Relation (L.Semiterm) :=
   .of_deltaOne (isSemitermDef_definable L) _ _
 
-def Language.TermSeq (n m w : V) : Prop := Seq w ∧ n = lh w ∧ ∀ i u, ⟪i, u⟫ ∈ w → L.IsSemiterm m u
+def Language.TermSeq (n m w : V) : Prop := Seq w ∧ n = lh w ∧ ∀ i u, ⟪i, u⟫ ∈ w → L.Semiterm m u
 
 variable {L}
 
@@ -167,19 +167,19 @@ protected lemma Language.TermSeq.seq {n m w : V} (h : L.TermSeq n m w) : Seq w :
 
 protected lemma Language.TermSeq.lh {n m w : V} (h : L.TermSeq n m w) : n = lh w := h.2.1
 
-lemma Language.TermSeq.prop {n m w : V} (h : L.TermSeq n m w) : ∀ i u, ⟪i, u⟫ ∈ w → L.IsSemiterm m u := h.2.2
+lemma Language.TermSeq.prop {n m w : V} (h : L.TermSeq n m w) : ∀ i u, ⟪i, u⟫ ∈ w → L.Semiterm m u := h.2.2
 
 lemma Language.TermSeq.prop_nth {n m w : V} (h : L.TermSeq n m w) {i} (hi : i < n) :
-    L.IsSemiterm m (h.seq.nth (by simpa [←h.lh] using hi)) := h.prop i _ (by simp)
+    L.Semiterm m (h.seq.nth (by simpa [←h.lh] using hi)) := h.prop i _ (by simp)
 
-lemma Language.TermSeq.seqCons {n m w t : V} (h : L.TermSeq n m w) (ht : L.IsSemiterm m t) : L.TermSeq (n + 1) m (w ⁀' t) :=
+lemma Language.TermSeq.seqCons {n m w t : V} (h : L.TermSeq n m w) (ht : L.Semiterm m t) : L.TermSeq (n + 1) m (w ⁀' t) :=
   ⟨h.seq.seqCons t, by simp [h.seq, h.lh], fun i u hi ↦ by
     rcases mem_seqCons_iff.mp hi with (⟨rfl, rfl⟩ | hi); { exact ht }; { exact h.prop _ _ hi }⟩
 
 section
 
 private lemma termSeq_iff (n m w : V) :
-    L.TermSeq n m w ↔ Seq w ∧ n = lh w ∧ ∀ i < w, ∀ u < w, ⟪i, u⟫ ∈ w → L.IsSemiterm m u :=
+    L.TermSeq n m w ↔ Seq w ∧ n = lh w ∧ ∀ i < w, ∀ u < w, ⟪i, u⟫ ∈ w → L.Semiterm m u :=
   ⟨fun h ↦ ⟨Language.TermSeq.seq h, Language.TermSeq.lh h, fun i _ u _ hi ↦ Language.TermSeq.prop h i u hi⟩,
    by rintro ⟨Sw, hn, h⟩
       exact ⟨by simpa using Sw, by simpa using hn,
@@ -211,28 +211,28 @@ end
 
 variable {n : V}
 
-local prefix:80 "𝐓ⁿ " => L.IsSemiterm n
+local prefix:80 "𝐓ⁿ " => L.Semiterm n
 
-lemma Language.IsSemiterm.case_iff {t : V} :
+lemma Language.Semiterm.case_iff {t : V} :
     𝐓ⁿ t ↔
     (∃ z < n, t = ^#z) ∨
     (∃ x, t = ^&x) ∨
     (∃ k f v : V, L.Func k f ∧ L.TermSeq k n v ∧ t = ^func k f v) := by
   simpa [construction, Phi, TermSeq, and_assoc] using (construction L).case
 
-alias ⟨Language.IsSemiterm.case, Language.IsSemiterm.mk⟩ := Language.IsSemiterm.case_iff
+alias ⟨Language.Semiterm.case, Language.Semiterm.mk⟩ := Language.Semiterm.case_iff
 
-@[simp] lemma Language.IsSemiterm.bvar {z : V} : 𝐓ⁿ ^#z ↔ z < n :=
+@[simp] lemma Language.Semiterm.bvar {z : V} : 𝐓ⁿ ^#z ↔ z < n :=
   ⟨by intro h
       rcases h.case with (⟨z', hz, hzz'⟩ | ⟨x, h⟩ | ⟨k, f, v, _, _, h⟩)
       · rcases (show z = z' from by simpa using hzz'); exact hz
       · simp [qqBvar, qqFvar] at h
       · simp [qqBvar, qqFunc] at h,
-    fun hz ↦ Language.IsSemiterm.mk (Or.inl ⟨z, hz, rfl⟩)⟩
+    fun hz ↦ Language.Semiterm.mk (Or.inl ⟨z, hz, rfl⟩)⟩
 
-@[simp] lemma Language.IsSemiterm.fvar (x : V) : 𝐓ⁿ ^&x := Language.IsSemiterm.mk (Or.inr <| Or.inl ⟨x, rfl⟩)
+@[simp] lemma Language.Semiterm.fvar (x : V) : 𝐓ⁿ ^&x := Language.Semiterm.mk (Or.inr <| Or.inl ⟨x, rfl⟩)
 
-@[simp] lemma Language.IsSemiterm.func_iff {k f v : V} :
+@[simp] lemma Language.Semiterm.func_iff {k f v : V} :
     𝐓ⁿ (^func k f v) ↔ L.Func k f ∧ L.TermSeq k n v :=
   ⟨by intro h
       rcases h.case with (⟨_, _, h⟩ | ⟨x, h⟩ | ⟨k', f', v', hkf, ⟨Sv, hk, hv⟩, h⟩)
@@ -240,12 +240,12 @@ alias ⟨Language.IsSemiterm.case, Language.IsSemiterm.mk⟩ := Language.IsSemit
       · simp [qqFunc, qqFvar] at h
       · rcases (show k = k' ∧ f = f' ∧ v = v' by simpa [qqFunc] using h) with ⟨rfl, rfl, rfl⟩
         exact ⟨hkf, Sv, hk, hv⟩,
-   by rintro ⟨hkf, Sv, hk, hv⟩; exact Language.IsSemiterm.mk (Or.inr <| Or.inr ⟨k, f, v, hkf, ⟨Sv, hk, hv⟩, rfl⟩)⟩
+   by rintro ⟨hkf, Sv, hk, hv⟩; exact Language.Semiterm.mk (Or.inr <| Or.inr ⟨k, f, v, hkf, ⟨Sv, hk, hv⟩, rfl⟩)⟩
 
-lemma Language.IsSemiterm.func {k f v : V} (hkf : L.Func k f) (hv : L.TermSeq k n v) :
-    𝐓ⁿ (^func k f v) := Language.IsSemiterm.func_iff.mpr ⟨hkf, hv⟩
+lemma Language.Semiterm.func {k f v : V} (hkf : L.Func k f) (hv : L.TermSeq k n v) :
+    𝐓ⁿ (^func k f v) := Language.Semiterm.func_iff.mpr ⟨hkf, hv⟩
 
-lemma Language.IsSemiterm.induction (Γ) {P : V → Prop} (hP : (Γ, 1)-Predicate P)
+lemma Language.Semiterm.induction (Γ) {P : V → Prop} (hP : (Γ, 1)-Predicate P)
     (hbvar : ∀ z < n, P (^#z)) (hfvar : ∀ x, P (^&x))
     (hfunc : ∀ k f v, L.Func k f → L.TermSeq k n v → (∀ i u, ⟪i, u⟫ ∈ v → P u) → P (^func k f v)) :
     ∀ t, 𝐓ⁿ t → P t :=
@@ -316,7 +316,7 @@ namespace Construction
 variable {arity : ℕ} {β : Blueprint pL arity} (c : Construction V L β)
 
 def Phi (param : Fin arity → V) (n : V) (C : Set V) (pr : V) : Prop :=
-  L.IsSemiterm n (π₁ pr) ∧ (
+  L.Semiterm n (π₁ pr) ∧ (
   (∃ z, pr = ⟪^#z, c.bvar param n z⟫) ∨
   (∃ x, pr = ⟪^&x, c.fvar param n x⟫) ∨
   (∃ k f v v', (Seq v' ∧ k = lh v' ∧ ∀ i z z', ⟪i, z⟫ ∈ v → ⟪i, z'⟫ ∈ v' → ⟪z, z'⟫ ∈ C) ∧ pr = ⟪^func k f v, c.func param n k f v v'⟫))
@@ -330,7 +330,7 @@ lemma seq_bound {k s m : V} (Ss : Seq s) (hk : k = lh s) (hs : ∀ i z, ⟪i, z�
 
 private lemma phi_iff (param : Fin arity → V) (n C pr : V) :
     c.Phi param n {x | x ∈ C} pr ↔
-    ∃ t ≤ pr, ∃ y ≤ pr, pr = ⟪t, y⟫ ∧ L.IsSemiterm n t ∧ (
+    ∃ t ≤ pr, ∃ y ≤ pr, pr = ⟪t, y⟫ ∧ L.Semiterm n t ∧ (
       (∃ z < t, t = ^#z ∧ y = c.bvar param n z) ∨
       (∃ x < t, t = ^&x ∧ y = c.fvar param n x) ∨
       (∃ k < t, ∃ f < t, ∃ v < t, ∃ e, e = exp ((k + C + 1)^2) ∧ ∃ v' < e,
@@ -447,7 +447,7 @@ variable {c}
 
 lemma Graph.case_iff {t y : V} :
     c.Graph param n t y ↔
-    L.IsSemiterm n t ∧
+    L.Semiterm n t ∧
     ( (∃ z, t = ^#z ∧ y = c.bvar param n z) ∨
       (∃ x, t = ^&x ∧ y = c.fvar param n x) ∨
       (∃ k f v v', (Seq v' ∧ k = lh v' ∧ ∀ i z z', ⟪i, z⟫ ∈ v → ⟪i, z'⟫ ∈ v' → c.Graph param n z z') ∧
@@ -473,7 +473,7 @@ instance termSubst_definable : Arith.Definable ℒₒᵣ 𝚺₁ (fun v ↦ c.Gr
   simpa using Definable.retractiont (n := 2) (termSubst_definable c) (&n :> #0 :> #1 :> fun i ↦ &(param i))
 
 lemma graph_dom_isSemiterm {t y} :
-    c.Graph param n t y → L.IsSemiterm n t := fun h ↦ Graph.case_iff.mp h |>.1
+    c.Graph param n t y → L.Semiterm n t := fun h ↦ Graph.case_iff.mp h |>.1
 
 lemma graph_bvar_iff {z} (hz : z < n) :
     c.Graph param n ^#z y ↔ y = c.bvar param n z := by
@@ -513,8 +513,8 @@ lemma graph_func_inv {n k f v y} :
 
 variable {c} (param n)
 
-lemma graph_exists {t : V} : L.IsSemiterm n t → ∃ y, c.Graph param n t y := by
-  apply Language.IsSemiterm.induction 𝚺 (P := fun t ↦ ∃ y, c.Graph param n t y) (by definability)
+lemma graph_exists {t : V} : L.Semiterm n t → ∃ y, c.Graph param n t y := by
+  apply Language.Semiterm.induction 𝚺 (P := fun t ↦ ∃ y, c.Graph param n t y) (by definability)
   case hbvar =>
     intro z hz; exact ⟨c.bvar param n z, by simp [c.graph_bvar_iff hz]⟩
   case hfvar =>
@@ -533,10 +533,10 @@ lemma graph_exists {t : V} : L.IsSemiterm n t → ∃ y, c.Graph param n t y := 
 
 lemma graph_unique {t y₁ y₂ : V} : c.Graph param n t y₁ → c.Graph param n t y₂ → y₁ = y₂ := by
   revert y₁ y₂
-  suffices L.IsSemiterm n t → ∀ y₁ y₂, c.Graph param n t y₁ → c.Graph param n t y₂ → y₁ = y₂
+  suffices L.Semiterm n t → ∀ y₁ y₂, c.Graph param n t y₁ → c.Graph param n t y₂ → y₁ = y₂
   by intro u₁ u₂ h₁ h₂; exact this (c.graph_dom_isSemiterm h₁) u₁ u₂ h₁ h₂
   intro ht
-  apply Language.IsSemiterm.induction 𝚷 ?_ ?_ ?_ ?_ t ht
+  apply Language.Semiterm.induction 𝚷 ?_ ?_ ?_ ?_ t ht
   · definability
   · intro z hz; simp [c.graph_bvar_iff hz]
   · intro x; simp [c.graph_fvar_iff]
@@ -552,25 +552,25 @@ lemma graph_unique {t y₁ y₂ : V} : c.Graph param n t y₁ → c.Graph param 
 
 variable (c)
 
-lemma graph_existsUnique {t : V} (ht : L.IsSemiterm n t) : ∃! y, c.Graph param n t y := by
+lemma graph_existsUnique {t : V} (ht : L.Semiterm n t) : ∃! y, c.Graph param n t y := by
   rcases graph_exists param n ht with ⟨y, hy⟩
   exact ExistsUnique.intro y hy (fun y' h' ↦ graph_unique param n h' hy)
 
 lemma graph_existsUnique_total (t : V) : ∃! y,
-    (L.IsSemiterm n t → c.Graph param n t y) ∧ (¬L.IsSemiterm n t → y = 0) := by
-  by_cases ht : L.IsSemiterm n t <;> simp [ht]; exact c.graph_existsUnique _ _ ht
+    (L.Semiterm n t → c.Graph param n t y) ∧ (¬L.Semiterm n t → y = 0) := by
+  by_cases ht : L.Semiterm n t <;> simp [ht]; exact c.graph_existsUnique _ _ ht
 
 def result (t : V) : V := Classical.choose! (c.graph_existsUnique_total param n t)
 
-def result_prop {t : V} (ht : L.IsSemiterm n t) : c.Graph param n t (c.result param n t) :=
+def result_prop {t : V} (ht : L.Semiterm n t) : c.Graph param n t (c.result param n t) :=
   Classical.choose!_spec (c.graph_existsUnique_total param n t) |>.1 ht
 
-def result_prop_not {t : V} (ht : ¬L.IsSemiterm n t) : c.result param n t = 0 :=
+def result_prop_not {t : V} (ht : ¬L.Semiterm n t) : c.result param n t = 0 :=
   Classical.choose!_spec (c.graph_existsUnique_total param n t) |>.2 ht
 
 variable {c param n}
 
-lemma result_eq_of_graph {t y} (ht : L.IsSemiterm n t) (h : c.Graph param n t y) :
+lemma result_eq_of_graph {t y} (ht : L.Semiterm n t) (h : c.Graph param n t y) :
     c.result param n t = y := Eq.symm <| Classical.choose_uniq (c.graph_existsUnique_total param n t) (by simp [h, ht])
 
 @[simp] lemma result_bvar {z} (hz : z < n) : c.result param n (^#z) = c.bvar param n z :=
@@ -638,7 +638,7 @@ def resultSeq_mem {k n w i z : V} (hw : L.TermSeq k n w)
 @[simp] def resultSeq_of_not {k n w : V} (hw : ¬L.TermSeq k n w) : c.resultSeq param k n w = 0 :=
   Classical.choose!_spec (c.graph_existsUnique_vec_total param k n w) |>.2 hw
 
-def resultSeq_seqCons {k n w t : V} (hw : L.TermSeq k n w) (ht : L.IsSemiterm n t) :
+def resultSeq_seqCons {k n w t : V} (hw : L.TermSeq k n w) (ht : L.Semiterm n t) :
     c.resultSeq param (k + 1) n (w ⁀' t) = c.resultSeq param k n w ⁀' c.result param n t :=
   Seq.lh_ext (c.resultSeq_seq param (hw.seqCons ht)) (Seq.seqCons (by simp [hw]) _) (by simp [hw, hw.seqCons ht]) (by
     intro i y₁ y₂ h₁ h₂
@@ -701,583 +701,6 @@ end
 end Construction
 
 end Language.TermRec
-
-/-
-section termSubst
-
-namespace FormalizedTermSubst
-
-variable (L)
-
-def Phi (n m w : V) (C : Set V) (p : V) : Prop :=
-  L.IsSemiterm n (π₁ p) ∧ L.IsSemiterm m (π₂ p) ∧
-  ( (∃ z < n, π₁ p = ^#z ∧ ⟪z, π₂ p⟫ ∈ w) ∨
-    (∃ x, π₁ p = ^&x ∧ π₂ p = ^&x) ∨
-    (∃ k f v v', π₁ p = ^func k f v ∧ π₂ p = ^func k f v' ∧ ∀ i u u', ⟪i, u⟫ ∈ v → ⟪i, u'⟫ ∈ v' → ⟪u, u'⟫ ∈ C) )
-
-private lemma phi_iff (n m w C p : V) :
-    Phi L n m w {x | x ∈ C} p ↔
-    ∃ t₁ ≤ p, ∃ t₂ ≤ p, p = ⟪t₁, t₂⟫ ∧ L.IsSemiterm n t₁ ∧ L.IsSemiterm m t₂ ∧
-    ( (∃ z < n, t₁ = ^#z ∧ ⟪z, t₂⟫ ∈ w) ∨
-      (∃ x < t₁, t₁ = ^&x ∧ t₂ = ^&x) ∨
-      (∃ k < t₁, ∃ f < t₁, ∃ v < t₁, ∃ v' < t₂, t₁ = ^func k f v ∧ t₂ = ^func k f v' ∧
-        (∀ i < v, ∀ u < v, ∀ u' < v', ⟪i, u⟫ ∈ v → ⟪i, u'⟫ ∈ v' → ⟪u, u'⟫ ∈ C)) ) := by
-  constructor
-  ·{intro ⟨hp₁, hp₂, h⟩
-    refine ⟨π₁ p, by simp, π₂ p, by simp, by simp, hp₁, hp₂, ?_⟩
-    rcases h with (⟨z, hz, h₁, h⟩ | ⟨x, h₁, h₂⟩ | ⟨k, f, v, v', h₁, h₂, h⟩)
-    · left; exact ⟨z, hz, h₁, h⟩
-    · right; left; exact ⟨x, by simp [h₁], h₁, h₂⟩
-    · right; right
-      exact ⟨k, by simp [h₁], f, by simp [h₁], v, by simp [h₁], v', by simp [h₂],
-        h₁, h₂, fun i _ u _ u' _ hi hi' ↦ h i u u' hi hi'⟩}
-  · rintro ⟨t₁, _, t₂, _, rfl, ht₁, ht₂, h⟩
-    refine ⟨by simpa using ht₁, by simpa using ht₂, ?_⟩
-    rcases h with (⟨z, hz, rfl, h⟩ | ⟨x, _, rfl, rfl⟩ | ⟨k, _, f, _, v, _, v', _, rfl, rfl, h⟩)
-    · left; exact ⟨z, hz, by simp [h]⟩
-    · right; left; exact ⟨x, by simp⟩
-    · right; right
-      exact ⟨k, f, v, v', by simp, by simp, fun i u u' hi hi' ↦
-        h i (lt_of_mem_dom hi) u (lt_of_mem_rng hi) u' (lt_of_mem_rng hi') hi hi'⟩
-
-def formulaAux : Semisentence ℒₒᵣ 7 := “t₁ t₂ p C n m w |
-  (∃ z < n, !qqBvarDef t₁ z ∧ z ~[w] t₂) ∨
-  (∃ x < t₁, !qqFvarDef t₁ x ∧ !qqFvarDef t₂ x) ∨
-  (∃ k < t₁, ∃ f < t₁, ∃ v < t₁, ∃ v' < t₂, !qqFuncDef t₁ k f v ∧ !qqFuncDef t₂ k f v' ∧
-  (∀ i < v, ∀ u < v, ∀ u' < v', i ~[v] u → i ~[v'] u' → u ~[C] u'))”
-
-def formula (pL : LDef) : Fixpoint.Blueprint 3 := ⟨.mkDelta
-  (.mkSigma
-    “p C n m w |
-      ∃ t₁ <⁺ p, ∃ t₂ <⁺ p, !pairDef p t₁ t₂ ∧ !pL.isSemitermDef.sigma n t₁ ∧ !pL.isSemitermDef.sigma m t₂ ∧
-      !formulaAux t₁ t₂ p C n m w”
-    (by simp [formulaAux]))
-  (.mkPi
-    “p C n m w |
-      ∃ t₁ <⁺ p, ∃ t₂ <⁺ p, !pairDef p t₁ t₂ ∧ !pL.isSemitermDef.pi n t₁ ∧ !pL.isSemitermDef.pi m t₂ ∧
-      !formulaAux t₁ t₂ p C n m w”
-    (by simp [formulaAux]))⟩
-
-def construction : Fixpoint.Construction V (formula pL) where
-  Φ := fun v ↦ Phi L (v 0) (v 1) (v 2)
-  defined := ⟨fun v ↦
-    by simp [formula, HSemiformula.val_sigma, eval_isSemitermDef L, (isSemiterm_defined L).proper.iff'],
-  fun v ↦ by simpa [formula, HSemiformula.val_sigma, eval_isSemitermDef L, formulaAux] using phi_iff _ _ _ _ _ _⟩
-  monotone := by
-    rintro C C' hC v p ⟨ht₁, ht₂, (h | h | ⟨k, f, v, v', h₁, h₂, h⟩)⟩
-    · exact ⟨ht₁, ht₂, Or.inl h⟩
-    · exact ⟨ht₁, ht₂, Or.inr <| Or.inl h⟩
-    · exact ⟨ht₁, ht₂, Or.inr <| Or.inr ⟨k, f, v, v', h₁, h₂, fun i u u' hi hi' ↦ hC (h i u u' hi hi')⟩⟩
-
-instance : (construction L).StrongFinite V where
-  strong_finite := by
-    rintro C v p ⟨ht₁, ht₂, (h | h | ⟨k, f, v, v', h₁, h₂, h⟩)⟩
-    · exact ⟨ht₁, ht₂, Or.inl h⟩
-    · exact ⟨ht₁, ht₂, Or.inr <| Or.inl h⟩
-    · exact ⟨ht₁, ht₂, Or.inr <| Or.inr ⟨k, f, v, v', h₁, h₂, fun i u u' hi hi' ↦ ⟨h i u u' hi hi', by
-      have : ⟪u, u'⟫ < ⟪π₁ p, π₂ p⟫ := pair_lt_pair (by simpa [h₁] using lt_qqFunc_of_mem hi) (by simpa [h₂] using lt_qqFunc_of_mem hi')
-      simpa using this⟩⟩⟩
-
-def Subst (n m w : V) : V → Prop := (construction L).Fixpoint ![n, m, w]
-
-def _root_.LO.FirstOrder.Arith.LDef.substDef (pL : LDef) : 𝚫₁-Semisentence 4 :=
-  (formula pL).fixpointDefΔ₁.rew <| Rew.substs ![#3, #0, #1, #2]
-
-lemma subst_defined : 𝚫₁-Relation₄ (Subst L) via pL.substDef :=
-  ⟨HSemiformula.ProperOn.rew (construction L).fixpoint_definedΔ₁.proper _,
-   by intro v; simp [LDef.substDef, (construction L).eval_fixpointDefΔ₁, Subst]⟩
-
-@[simp] lemma eval_substDef (v) :
-    Semiformula.Evalbm V v pL.substDef.val ↔ Subst L (v 0) (v 1) (v 2) (v 3) := (subst_defined L).df.iff v
-
-instance subst_definable : 𝚫₁-Relation₄ (Subst L) := Defined.to_definable _ (subst_defined L)
-
-@[simp, definability] instance subst_definable' (Γ) : (Γ, m + 1)-Relation₄ (Subst L) :=
-  .of_deltaOne (subst_definable L) _ _
-
-variable {L}
-
-lemma Subst.case_iff {n m w p : V} :
-    Subst L n m w p ↔
-    L.IsSemiterm n (π₁ p) ∧ L.IsSemiterm m (π₂ p) ∧
-    ( (∃ z < n, π₁ p = ^#z ∧ ⟪z, π₂ p⟫ ∈ w) ∨
-      (∃ x, π₁ p = ^&x ∧ π₂ p = ^&x) ∨
-      (∃ k f v v', π₁ p = ^func k f v ∧ π₂ p = ^func k f v' ∧ ∀ i u u', ⟪i, u⟫ ∈ v → ⟪i, u'⟫ ∈ v' → Subst L n m w ⟪u, u'⟫) ) :=
-  (construction L).case
-
-alias ⟨Subst.case, Subst.mk⟩ := Subst.case_iff
-
-lemma Subst.semiterm₁ {n m w t t'} (h : Subst L n m w ⟪t, t'⟫) : L.IsSemiterm n t := by simpa using h.case.1
-
-lemma Subst.semiterm₂ {n m w t t'} (h : Subst L n m w ⟪t, t'⟫) : L.IsSemiterm m t' := by simpa using h.case.2.1
-
-lemma Subst.bvar {n m w z u : V} (hz : z < n) (hu : L.IsSemiterm m u) (h : ⟪z, u⟫ ∈ w) :
-    Subst L n m w ⟪^#z, u⟫ := Subst.mk ⟨by simp [hz], by simpa using hu, Or.inl ⟨z, hz, by simpa using h⟩⟩
-
-lemma Subst.bvar_iff {n m w z u : V} :
-    Subst L n m w ⟪^#z, u⟫ ↔ z < n ∧ L.IsSemiterm m u ∧ ⟪z, u⟫ ∈ w :=
-  ⟨by intro h
-      rcases h.case with ⟨_, hu, (⟨z', hz', hzz', h⟩ | ⟨x, h, _⟩ | ⟨k, f, v, v', h, _⟩)⟩
-      · rcases (show z = z' from by simpa using hzz'); exact ⟨hz', by simpa using hu, by simpa using h⟩
-      · simp [qqBvar, qqFvar] at h
-      · simp [qqBvar, qqFunc] at h,
-   by rintro ⟨hz, Hu, h⟩; exact Subst.bvar hz Hu h⟩
-
-@[simp] lemma Subst.fvar {n m w x : V} :
-    Subst L n m w ⟪^&x, ^&x⟫ := Subst.mk ⟨by simp, by simp, Or.inr <| Or.inl ⟨x, by simp⟩⟩
-
-lemma Subst.fvar_iff {n m w x u : V} :
-    Subst L n m w ⟪^&x, u⟫ ↔ u = ^&x := by
-  constructor
-  · intro h
-    rcases h.case with ⟨_, _, (⟨_, _, h, _⟩ | ⟨x', hx', h⟩ | ⟨_, _, _, _, h, _⟩)⟩
-    · simp [qqBvar, qqFvar] at h
-    · rcases (show x = x' from by simpa using hx'); simpa using h
-    · simp [qqFvar, qqFunc] at h
-  · rintro rfl; simp
-
-lemma Subst.func {n m w k f v v' : V}
-    (hkf : L.Func k f)
-    (hv : L.TermSeq k n v)
-    (hv' : L.TermSeq k m v')
-    (H : ∀ i u u', ⟪i, u⟫ ∈ v → ⟪i, u'⟫ ∈ v' → Subst L n m w ⟪u, u'⟫) :
-    Subst L n m w ⟪^func k f v, ^func k f v'⟫ :=
-  Subst.mk ⟨
-    by rw [pi₁_pair]; exact IsSemiterm.func hkf hv,
-    by rw [pi₂_pair]; exact IsSemiterm.func hkf hv',
-    Or.inr <| Or.inr ⟨k, f, v, v', by simp, by simp, H⟩⟩
-
-lemma Subst.func' {n m w k f v u : V} (h : Subst L n m w ⟪^func k f v, u⟫) :
-    ∃ v', Seq v' ∧ k = lh v' ∧ (∀ i u u', ⟪i, u⟫ ∈ v → ⟪i, u'⟫ ∈ v' → Subst L n m w ⟪u, u'⟫) ∧ u = ^func k f v' := by
-  rcases h.case with ⟨_, hu, (⟨_, _, h, _⟩ | ⟨x, h, _⟩ | ⟨k', f', v', v'', h₁, h₂, hv⟩)⟩
-  · simp [qqFunc, qqBvar] at h
-  · simp [qqFunc, qqFvar] at h
-  · rcases (show k = k' ∧ f = f' ∧ v = v' by simpa [qqFunc] using h₁) with ⟨rfl, rfl, rfl⟩
-    rcases (show u = ^func k f v'' by simpa using h₂)
-    have : L.Func k f ∧ Seq v'' ∧ k = lh v'' ∧ ∀ i u, ⟪i, u⟫ ∈ v'' → L.IsSemiterm m u := by simpa [IsSemiterm.func_iff] using hu
-    rcases this with ⟨_, Sv'', hk'', _⟩
-    exact ⟨v'', Sv'', hk'', hv, rfl⟩
-
-variable {n m w} (TSw : L.TermSeq n m w)
-
-lemma Subst.rng_exists {t : V} (ht : L.IsSemiterm n t) : ∃ u, Subst L n m w ⟪t, u⟫ := by
-  apply IsSemiterm.induction 𝚺 ?_ ?_ ?_ ?_ t ht
-  · definability
-  · intro z hz
-    have : ∃ u, ⟪z, u⟫ ∈ w := TSw.seq.exists (show z < lh w by simpa [TSw.lh] using hz)
-    rcases this with ⟨u, hu⟩
-    exact ⟨u, Subst.bvar hz (TSw.prop z u hu) hu⟩
-  · intro x; exact ⟨^&x, by simp⟩
-  · rintro k f v hkf hv ih
-    have : ∃ v', Seq v' ∧ lh v' = lh v ∧ ∀ i u', ⟪i, u'⟫ ∈ v' → ∀ u, ⟪i, u⟫ ∈ v → Subst L n m w ⟪u, u'⟫ := by
-      have : ∀ i < lh v, ∃ u', ∀ u, ⟪i, u⟫ ∈ v → Subst L n m w ⟪u, u'⟫ := by
-        intro i hi
-        have : ∃ u, Subst L n m w ⟪hv.seq.nth hi, u⟫ := ih i (hv.seq.nth hi) (by simp)
-        rcases this with ⟨u', hu'⟩
-        exact ⟨u', fun u hiuv  ↦ by rcases hv.seq.nth_uniq hi hiuv; exact hu'⟩
-      exact sigmaOne_skolem_seq
-        (by have : 𝚺₁-Relation fun x y ↦ ∀ u < v, ⟪x, u⟫ ∈ v → Subst L n m w ⟪u, y⟫ := by definability
-            exact this.of_iff fun w ↦ ⟨fun h u _ ↦ h u, fun h u hv ↦ h u (lt_of_mem_rng hv) hv⟩)
-        this
-    rcases this with ⟨v', Sv', hvv', h⟩
-    exact ⟨^func k f v',
-      Subst.func hkf hv ⟨Sv', by simp [hvv', hv.lh],
-        (fun i u' hi ↦ by
-          have : i < lh v := by simpa [hvv'] using Sv'.lt_lh_of_mem hi
-          exact h i u' hi (hv.seq.nth this) (by simp) |>.semiterm₂)⟩
-        (fun i u u' hi hi' ↦ h i u' hi' u hi)⟩
-
-lemma Subst.rng_unique
-    {t u₁ u₂ : V} : Subst L n m w ⟪t, u₁⟫ → Subst L n m w ⟪t, u₂⟫ → u₁ = u₂ := by
-  revert u₁ u₂
-  suffices L.IsSemiterm n t → ∀ u₁ u₂, Subst L n m w ⟪t, u₁⟫ → Subst L n m w ⟪t, u₂⟫ → u₁ = u₂
-  by intro u₁ u₂ h₁ h₂; exact this h₁.semiterm₁ u₁ u₂ h₁ h₂
-  intro ht
-  apply IsSemiterm.induction 𝚷 ?_ ?_ ?_ ?_ t ht
-  · definability
-  · simp only [bvar_iff, and_imp]
-    intro z _ u₁ u₂ _ _ h₁ _ _ h₂
-    exact TSw.seq.isMapping.uniq h₁ h₂
-  · simp [Subst.fvar_iff]
-  · intro k f v _ hv ih u₁ u₂ h₁ h₂
-    rcases Subst.func' h₁ with ⟨v₁, Sv₁, hk₁, hvv₁, rfl⟩
-    rcases Subst.func' h₂ with ⟨v₂, Sv₂, hk₂, hvv₂, rfl⟩
-    have : v₁ = v₂ := Sv₁.lh_ext Sv₂ (by simp [←hk₁, ←hk₂]) (by
-      intro i x₁ x₂ hxv₁ hxv₂
-      have hi : i < lh v := by simpa [←hv.lh, hk₁] using Sv₁.lt_lh_of_mem hxv₁
-      exact ih i (hv.seq.nth hi) (by simp) _ _ (hvv₁ _ _ _ (hv.seq.nth_mem hi) hxv₁) (hvv₂ _ _ _ (hv.seq.nth_mem hi) hxv₂))
-    rw [this]
-
-lemma Subst.rng_exists_unique {t : V} (ht : L.IsSemiterm n t) : ∃! u, Subst L n m w ⟪t, u⟫ := by
-  rcases Subst.rng_exists TSw ht with ⟨u, hu⟩
-  exact ExistsUnique.intro u hu (fun u' hu' ↦ Subst.rng_unique TSw hu' hu)
-
-variable (L)
-
-lemma Subst.rng_exists_unique_total (n m w t : V) :
-    ∃! u, (L.TermSeq n m w ∧ L.IsSemiterm n t → Subst L n m w ⟪t, u⟫) ∧ (¬(L.TermSeq n m w ∧ L.IsSemiterm n t) → u = 0) := by
-  by_cases h : L.TermSeq n m w ∧ L.IsSemiterm n t
-  · simp [h]; exact Subst.rng_exists_unique h.1 h.2
-  · simp [h]
-
-end FormalizedTermSubst
-
-open FormalizedTermSubst
-
-variable (L)
-
-def Language.termSubst (n m w t : V) : V := Classical.choose! (Subst.rng_exists_unique_total L n m w t)
-
-variable {L}
-
-def Language.TermSeq.spec_of_semiterm {n m w t : V} (TSw : L.TermSeq n m w) (ht : L.IsSemiterm n t) : Subst L n m w ⟪t, L.termSubst n m w t⟫ :=
-  Classical.choose!_spec (Subst.rng_exists_unique_total L n m w t) |>.1 ⟨TSw, ht⟩
-
-def Language.TermSeq.substs_isterm {n m w t : V} (TSw : L.TermSeq n m w) (ht : L.IsSemiterm n t) :
-    L.IsSemiterm m (L.termSubst n m w t) := TSw.spec_of_semiterm ht |>.semiterm₂
-
-def termSubst_spec {n m w t : V} :
-    ¬(L.TermSeq n m w ∧ L.IsSemiterm n t) → L.termSubst n m w t = 0 :=
-  Classical.choose!_spec (Subst.rng_exists_unique_total L n m w t) |>.2
-
-variable {n m w : V} (TSw : L.TermSeq n m w)
-
-lemma Language.TermSeq.termSubst_eq_of {t} (ht : L.IsSemiterm n t) (h : Subst L n m w ⟪t, u⟫) : L.termSubst n m w t = u :=
-  (TSw.spec_of_semiterm ht).rng_unique TSw h
-
-lemma termSubst_bvar {z : V} (hz : z < n) (hu : ⟪z, u⟫ ∈ w) : L.termSubst n m w (^#z) = u :=
-  TSw.termSubst_eq_of (by simp [hz]) (Subst.bvar hz (TSw.prop z u hu) hu)
-
-@[simp] lemma termSubst_fvar (x : V) : L.termSubst n m w (^&x) = ^&x :=
-  TSw.termSubst_eq_of (by simp) (by simp)
-
-lemma termSubst_func {k f v v' : V} (hfk : L.Func k f)
-    (hv : L.TermSeq k n v)
-    (hv' : L.TermSeq k m v')
-    (H : ∀ i u u', ⟪i, u⟫ ∈ v → ⟪i, u'⟫ ∈ v' → L.termSubst n m w u = u') : L.termSubst n m w (^func k f v) = ^func k f v' :=
-  TSw.termSubst_eq_of (IsSemiterm.func hfk hv)
-    (Subst.func hfk hv hv' (fun i u u' hi hi' ↦ by
-      rcases H i u u' hi hi'; exact TSw.spec_of_semiterm (hv.prop i u hi)))
-
-section
-
-variable (L)
-
-private lemma termSubst_graph (u n m w t : V) :
-    u = L.termSubst n m w t ↔
-    (L.TermSeq n m w ∧ L.IsSemiterm n t → ∃ p ≤ (t + u + 1)^2, p = ⟪t, u⟫ ∧ Subst L n m w p) ∧ (¬(L.TermSeq n m w ∧ L.IsSemiterm n t) → u = 0) :=
-  Iff.trans (Classical.choose!_eq_iff (Subst.rng_exists_unique_total L n m w t)) ⟨by
-    rintro ⟨hp, hn⟩
-    exact ⟨fun h ↦ ⟨⟪t, u⟫, by simp, rfl, hp h⟩, hn⟩, by
-    rintro ⟨hp, hn⟩
-    exact ⟨fun h ↦ by rcases hp h with ⟨_, _, rfl, h⟩; exact h, hn⟩⟩
-
-def _root_.LO.FirstOrder.Arith.LDef.termSubstDef (pL : LDef) : 𝚺₁-Semisentence 5 := .mkSigma
-  “u n m w t | (!pL.termSeqDef.pi n m w ∧ !pL.isSemitermDef.pi n t → ∃ p <⁺ (t + u + 1)², !pairDef p t u ∧ !pL.substDef.sigma n m w p) ∧
-    (¬(!pL.termSeqDef.sigma n m w ∧ !pL.isSemitermDef.sigma n t) → u = 0)” (by simp)
-
-lemma termSubst_defined : 𝚺₁-Function₄ L.termSubst via pL.termSubstDef := by
-  intro v
-  simp [LDef.termSubstDef, termSubst_graph, HSemiformula.val_sigma, eval_termSeq L,
-    eval_isSemitermDef L, (termSeq_defined L).proper.iff', (isSemiterm_defined L).proper.iff', eval_substDef L, -and_imp, -not_and]
-  apply iff_of_eq; congr; simp [imp_iff_not_or]; rfl
-
-@[simp] lemma termSubst_defined_iff (v : Fin 5 → V) :
-    Semiformula.Evalbm (L := ℒₒᵣ) V v pL.termSubstDef ↔ v 0 = L.termSubst (v 1) (v 2) (v 3) (v 4) := (termSubst_defined L).df.iff v
-
-instance termSubst_definable : 𝚺₁-Function₄ L.termSubst :=
-  Defined.to_definable _ (termSubst_defined L)
-/-
-@[simp, definability] instance termSubst_definable' (Γ m) : (Γ, m + 1)-Function₄ L.termSubst :=
-  .of_sigmaOne (termSubst_definable L) _ _
--/
-instance termSubst_definable₂ (n m) : 𝚺₁-Function₂ (L.termSubst n m) := by
-  simpa using DefinableFunction.retractiont (n := 2) (termSubst_definable L) ![&n, &m, #0, #1]
-
-@[simp, definability] instance termSubst_definable₂' (Γ l n m) : (Γ, l + 1)-Function₂ (L.termSubst n m) :=
-  .of_sigmaOne (termSubst_definable₂ L n m) _ _
-
-end
-
-end termSubst
-
-section termShift
-
-namespace FormalizedTermShift
-
-variable (L)
-
-def Phi (n : V) (C : Set V) (p : V) : Prop :=
-  L.IsSemiterm n (π₁ p) ∧ L.IsSemiterm n (π₂ p) ∧
-  ( (∃ z < n, π₁ p = ^#z ∧ π₂ p = ^#z) ∨
-    (∃ x, π₁ p = ^&x ∧ π₂ p = ^&(x + 1)) ∨
-    (∃ k f v v', π₁ p = ^func k f v ∧ π₂ p = ^func k f v' ∧ ∀ i u u', ⟪i, u⟫ ∈ v → ⟪i, u'⟫ ∈ v' → ⟪u, u'⟫ ∈ C) )
-
-private lemma phi_iff (n C p : V) :
-    Phi L n {x | x ∈ C} p ↔
-    ∃ t₁ ≤ p, ∃ t₂ ≤ p, p = ⟪t₁, t₂⟫ ∧ L.IsSemiterm n t₁ ∧ L.IsSemiterm n t₂ ∧
-    ( (∃ z < n, t₁ = ^#z ∧ t₂ = ^#z) ∨
-      (∃ x < t₁, t₁ = ^&x ∧ t₂ = ^&(x + 1)) ∨
-      (∃ k < t₁, ∃ f < t₁, ∃ v < t₁, ∃ v' < t₂, t₁ = ^func k f v ∧ t₂ = ^func k f v' ∧
-        (∀ i < v, ∀ u < v, ∀ u' < v', ⟪i, u⟫ ∈ v → ⟪i, u'⟫ ∈ v' → ⟪u, u'⟫ ∈ C)) ) := by
-  constructor
-  ·{intro ⟨hp₁, hp₂, h⟩
-    refine ⟨π₁ p, by simp, π₂ p, by simp, by simp, hp₁, hp₂, ?_⟩
-    rcases h with (⟨z, hz, h₁, h⟩ | ⟨x, h₁, h₂⟩ | ⟨k, f, v, v', h₁, h₂, h⟩)
-    · left; exact ⟨z, hz, h₁, h⟩
-    · right; left; exact ⟨x, by simp [h₁], h₁, h₂⟩
-    · right; right
-      exact ⟨k, by simp [h₁], f, by simp [h₁], v, by simp [h₁], v', by simp [h₂],
-        h₁, h₂, fun i _ u _ u' _ hi hi' ↦ h i u u' hi hi'⟩}
-  · rintro ⟨t₁, _, t₂, _, rfl, ht₁, ht₂, h⟩
-    refine ⟨by simpa using ht₁, by simpa using ht₂, ?_⟩
-    rcases h with (⟨z, hz, rfl, h⟩ | ⟨x, _, rfl, rfl⟩ | ⟨k, _, f, _, v, _, v', _, rfl, rfl, h⟩)
-    · left; exact ⟨z, hz, by simp [h]⟩
-    · right; left; exact ⟨x, by simp⟩
-    · right; right
-      exact ⟨k, f, v, v', by simp, by simp, fun i u u' hi hi' ↦
-        h i (lt_of_mem_dom hi) u (lt_of_mem_rng hi) u' (lt_of_mem_rng hi') hi hi'⟩
-
-def formulaAux : Semisentence ℒₒᵣ 5 := “t₁ t₂ p C n |
-  (∃ z < n, !qqBvarDef t₁ z ∧ !qqBvarDef t₂ z) ∨
-  (∃ x < t₁, !qqFvarDef t₁ x ∧ !qqFvarDef t₂ (x + 1)) ∨
-  (∃ k < t₁, ∃ f < t₁, ∃ v < t₁, ∃ v' < t₂, !qqFuncDef t₁ k f v ∧ !qqFuncDef t₂ k f v' ∧
-  (∀ i < v, ∀ u < v, ∀ u' < v', i ~[v] u → i ~[v'] u' → u ~[C] u'))”
-
-def formula (pL : LDef) : Fixpoint.Blueprint 1 := ⟨.mkDelta
-  (.mkSigma
-    “p C n |
-      ∃ t₁ <⁺ p, ∃ t₂ <⁺ p, !pairDef p t₁ t₂ ∧ !pL.isSemitermDef.sigma n t₁ ∧ !pL.isSemitermDef.sigma n t₂ ∧
-      !formulaAux t₁ t₂ p C n”
-    (by simp [formulaAux]))
-  (.mkPi
-    “p C n |
-      ∃ t₁ <⁺ p, ∃ t₂ <⁺ p, !pairDef p t₁ t₂ ∧ !pL.isSemitermDef.pi n t₁ ∧ !pL.isSemitermDef.pi n t₂ ∧
-      !formulaAux t₁ t₂ p C n”
-    (by simp [formulaAux]))⟩
-
-def construction : Fixpoint.Construction V (formula pL) where
-  Φ := fun v ↦ Phi L (v 0)
-  defined := ⟨fun v ↦
-    by simp [formula, HSemiformula.val_sigma, eval_isSemitermDef L, (isSemiterm_defined L).proper.iff'],
-  fun v ↦ by simpa [formula, HSemiformula.val_sigma, eval_isSemitermDef L, formulaAux] using phi_iff _ _ _ _⟩
-  monotone := by
-    rintro C C' hC v p ⟨ht₁, ht₂, (h | h | ⟨k, f, v, v', h₁, h₂, h⟩)⟩
-    · exact ⟨ht₁, ht₂, Or.inl h⟩
-    · exact ⟨ht₁, ht₂, Or.inr <| Or.inl h⟩
-    · exact ⟨ht₁, ht₂, Or.inr <| Or.inr ⟨k, f, v, v', h₁, h₂, fun i u u' hi hi' ↦ hC (h i u u' hi hi')⟩⟩
-
-instance : (construction L).StrongFinite V where
-  strong_finite := by
-    rintro C v p ⟨ht₁, ht₂, (h | h | ⟨k, f, v, v', h₁, h₂, h⟩)⟩
-    · exact ⟨ht₁, ht₂, Or.inl h⟩
-    · exact ⟨ht₁, ht₂, Or.inr <| Or.inl h⟩
-    · exact ⟨ht₁, ht₂, Or.inr <| Or.inr ⟨k, f, v, v', h₁, h₂, fun i u u' hi hi' ↦ ⟨h i u u' hi hi', by
-      have : ⟪u, u'⟫ < ⟪π₁ p, π₂ p⟫ := pair_lt_pair (by simpa [h₁] using lt_qqFunc_of_mem hi) (by simpa [h₂] using lt_qqFunc_of_mem hi')
-      simpa using this⟩⟩⟩
-
-def Shift (n : V) : V → Prop := (construction L).Fixpoint ![n]
-
-def shiftDef (pL : LDef) : 𝚫₁-Semisentence 2 := (formula pL).fixpointDefΔ₁.rew <| Rew.substs ![#1, #0]
-
-lemma shift_defined : 𝚫₁-Relation (Shift L) via (shiftDef pL) :=
-  ⟨HSemiformula.ProperOn.rew (construction L).fixpoint_definedΔ₁.proper _,
-   by intro v; simp [shiftDef, (construction L).eval_fixpointDefΔ₁, Shift]⟩
-
-@[simp] lemma eval_shiftDef (v) :
-    Semiformula.Evalbm V v (shiftDef pL).val ↔ Shift L (v 0) (v 1) := (shift_defined L).df.iff v
-
-instance shift_definable : 𝚫₁-Relation (Shift L) := Defined.to_definable _ (shift_defined L)
-
-@[simp, definability] instance shift_definable' (Γ) : (Γ, m + 1)-Relation (Shift L) :=
-  .of_deltaOne (shift_definable L) _ _
-
-variable {L}
-
-lemma Shift.case_iff {n p : V} :
-    Shift L n p ↔
-    L.IsSemiterm n (π₁ p) ∧ L.IsSemiterm n (π₂ p) ∧
-    ( (∃ z < n, π₁ p = ^#z ∧ π₂ p = ^#z) ∨
-      (∃ x, π₁ p = ^&x ∧ π₂ p = ^&(x + 1)) ∨
-      (∃ k f v v', π₁ p = ^func k f v ∧ π₂ p = ^func k f v' ∧ ∀ i u u', ⟪i, u⟫ ∈ v → ⟪i, u'⟫ ∈ v' → Shift L n ⟪u, u'⟫) ) :=
-  (construction L).case
-
-alias ⟨Shift.case, Shift.mk⟩ := Shift.case_iff
-
-lemma Shift.semiterm₁ {n t t'} (h : Shift L n ⟪t, t'⟫) : L.IsSemiterm n t := by simpa using h.case.1
-
-lemma Shift.semiterm₂ {n t t'} (h : Shift L n ⟪t, t'⟫) : L.IsSemiterm n t' := by simpa using h.case.2.1
-
-@[simp] lemma Shift.bvar {n z : V} (hz : z < n) :
-    Shift L n ⟪^#z, ^#z⟫ := Shift.mk ⟨by simp [hz], by simp [hz]⟩
-
-lemma Shift.bvar_iff {n z u : V} :
-    Shift L n ⟪^#z, u⟫ ↔ z < n ∧ u = ^#z :=
-  ⟨by intro h
-      rcases h.case with ⟨_, _, (⟨z', hz', hzz', h⟩ | ⟨x, h, _⟩ | ⟨k, f, v, v', h, _⟩)⟩
-      · rcases (show z = z' from by simpa using hzz'); exact ⟨hz', by simpa using h⟩
-      · simp [qqBvar, qqFvar] at h
-      · simp [qqBvar, qqFunc] at h,
-   by rintro ⟨hz, Hu, h⟩; exact Shift.bvar hz⟩
-
-@[simp] lemma Shift.fvar {n : V} (x : V):
-    Shift L n ⟪^&x, ^&(x + 1)⟫ := Shift.mk ⟨by simp, by simp⟩
-
-lemma Shift.fvar_iff {n x u : V} :
-    Shift L n ⟪^&x, u⟫ ↔ u = ^&(x + 1) :=
-  ⟨by intro h
-      rcases h.case with ⟨_, _, (⟨_, _, h, _⟩ | ⟨x', hx', h⟩ | ⟨_, _, _, _, h, _, _⟩)⟩
-      · simp [qqBvar, qqFvar] at h
-      · rcases (show x = x' by simpa using hx'); simpa using h
-      · simp [qqFvar, qqFunc] at h,
-   by rintro ⟨hz, Hu, h⟩; exact Shift.fvar x⟩
-
-lemma Shift.func {n k f v v' : V}
-    (hkf : L.Func k f)
-    (hv : L.TermSeq k n v)
-    (hv' : L.TermSeq k n v')
-    (H : ∀ i u u', ⟪i, u⟫ ∈ v → ⟪i, u'⟫ ∈ v' → Shift L n ⟪u, u'⟫) :
-    Shift L n ⟪^func k f v, ^func k f v'⟫ :=
-  Shift.mk ⟨
-    by rw [pi₁_pair]; exact IsSemiterm.func hkf hv,
-    by rw [pi₂_pair]; exact IsSemiterm.func hkf hv',
-    Or.inr <| Or.inr ⟨k, f, v, v', by simp, by simp, H⟩⟩
-
-lemma Shift.func' {n k f v u : V} (h : Shift L n ⟪^func k f v, u⟫) :
-    ∃ v', Seq v' ∧ k = lh v' ∧ (∀ i u u', ⟪i, u⟫ ∈ v → ⟪i, u'⟫ ∈ v' → Shift L n ⟪u, u'⟫) ∧ u = ^func k f v' := by
-  rcases h.case with ⟨_, hu, (⟨_, _, h, _⟩ | ⟨x, h, _⟩ | ⟨k', f', v', v'', h₁, h₂, hv⟩)⟩
-  · simp [qqFunc, qqBvar] at h
-  · simp [qqFunc, qqFvar] at h
-  · rcases (show k = k' ∧ f = f' ∧ v = v' by simpa [qqFunc] using h₁) with ⟨rfl, rfl, rfl⟩
-    rcases (show u = ^func k f v'' by simpa using h₂)
-    have : L.Func k f ∧ Seq v'' ∧ k = lh v'' ∧ ∀ i u, ⟪i, u⟫ ∈ v'' → L.IsSemiterm n u := by simpa [IsSemiterm.func_iff] using hu
-    rcases this with ⟨_, Sv'', hk'', _⟩
-    exact ⟨v'', Sv'', hk'', hv, rfl⟩
-
-variable {n : V}
-
-lemma Shift.rng_exists {t : V} (ht : L.IsSemiterm n t) : ∃ u, Shift L n ⟪t, u⟫ := by
-  apply IsSemiterm.induction 𝚺 ?_ ?_ ?_ ?_ t ht
-  · definability
-  · intro z hz; exact ⟨^#z, Shift.bvar hz⟩
-  · intro x; exact ⟨^&(x + 1), by simp⟩
-  · rintro k f v hkf hv ih
-    have : ∃ v', Seq v' ∧ lh v' = lh v ∧ ∀ i u', ⟪i, u'⟫ ∈ v' → ∀ u, ⟪i, u⟫ ∈ v → Shift L n ⟪u, u'⟫ := by
-      have : ∀ i < lh v, ∃ u', ∀ u, ⟪i, u⟫ ∈ v → Shift L n ⟪u, u'⟫ := by
-        intro i hi
-        have : ∃ u, Shift L n ⟪hv.seq.nth hi, u⟫ := ih i (hv.seq.nth hi) (by simp)
-        rcases this with ⟨u', hu'⟩
-        exact ⟨u', fun u hiuv  ↦ by rcases hv.seq.nth_uniq hi hiuv; exact hu'⟩
-      exact sigmaOne_skolem_seq
-        (by have : 𝚺₁-Relation fun x y ↦ ∀ u < v, ⟪x, u⟫ ∈ v → Shift L n ⟪u, y⟫ := by definability
-            exact this.of_iff fun w ↦ ⟨fun h u _ ↦ h u, fun h u hv ↦ h u (lt_of_mem_rng hv) hv⟩)
-        this
-    rcases this with ⟨v', Sv', hvv', h⟩
-    exact ⟨^func k f v',
-      Shift.func hkf hv ⟨Sv', by simp [hvv', hv.lh],
-        (fun i u' hi ↦ by
-          have : i < lh v := by simpa [hvv'] using Sv'.lt_lh_of_mem hi
-          exact h i u' hi (hv.seq.nth this) (by simp) |>.semiterm₂)⟩
-        (fun i u u' hi hi' ↦ h i u' hi' u hi)⟩
-
-lemma Shift.rng_unique
-    {t u₁ u₂ : V} : Shift L n ⟪t, u₁⟫ → Shift L n ⟪t, u₂⟫ → u₁ = u₂ := by
-  revert u₁ u₂
-  suffices L.IsSemiterm n t → ∀ u₁ u₂, Shift L n ⟪t, u₁⟫ → Shift L n ⟪t, u₂⟫ → u₁ = u₂
-  by intro u₁ u₂ h₁ h₂; exact this h₁.semiterm₁ u₁ u₂ h₁ h₂
-  intro ht
-  apply IsSemiterm.induction 𝚷 ?_ ?_ ?_ ?_ t ht
-  · definability
-  · simp only [bvar_iff, and_imp]
-    rintro z _ u₁ u₂ _ rfl _ rfl; rfl
-  · simp [Shift.fvar_iff]
-  · intro k f v _ hv ih u₁ u₂ h₁ h₂
-    rcases Shift.func' h₁ with ⟨v₁, Sv₁, hk₁, hvv₁, rfl⟩
-    rcases Shift.func' h₂ with ⟨v₂, Sv₂, hk₂, hvv₂, rfl⟩
-    have : v₁ = v₂ := Sv₁.lh_ext Sv₂ (by simp [←hk₁, ←hk₂]) (by
-      intro i x₁ x₂ hxv₁ hxv₂
-      have hi : i < lh v := by simpa [←hv.lh, hk₁] using Sv₁.lt_lh_of_mem hxv₁
-      exact ih i (hv.seq.nth hi) (by simp) _ _ (hvv₁ _ _ _ (hv.seq.nth_mem hi) hxv₁) (hvv₂ _ _ _ (hv.seq.nth_mem hi) hxv₂))
-    rw [this]
-
-lemma Shift.rng_exists_unique {t : V} (ht : L.IsSemiterm n t) : ∃! u, Shift L n ⟪t, u⟫ := by
-  rcases Shift.rng_exists ht with ⟨u, hu⟩
-  exact ExistsUnique.intro u hu (fun u' hu' ↦ Shift.rng_unique hu' hu)
-
-variable (L)
-
-lemma Shift.rng_exists_unique_total (n t : V) :
-    ∃! u, (L.IsSemiterm n t → Shift L n ⟪t, u⟫) ∧ (¬L.IsSemiterm n t → u = 0) := by
-  by_cases h : L.IsSemiterm n t
-  · simp [h]; exact Shift.rng_exists_unique h
-  · simp [h]
-
-end FormalizedTermShift
-
-open FormalizedTermShift
-
-variable (L)
-
-def Language.termShift (n t : V) : V := Classical.choose! (Shift.rng_exists_unique_total L n t)
-
-variable {L}
-
-lemma Language.IsSemiterm.termShift_spec {n t : V} (ht : L.IsSemiterm n t) : Shift L n ⟪t, L.termShift n t⟫ :=
-  Classical.choose!_spec (Shift.rng_exists_unique_total L n t) |>.1 ht
-
-lemma termShift_spec_of_not_termShift {n t : V} :
-    ¬L.IsSemiterm n t → L.termShift n t = 0 :=
-  Classical.choose!_spec (Shift.rng_exists_unique_total L n t) |>.2
-
-lemma Language.IsSemiterm.termShift_eq_of {n t} (ht : L.IsSemiterm n t) (h : Shift L n ⟪t, u⟫) : L.termShift n t = u :=
-  ht.termShift_spec.rng_unique h
-
-lemma termShift_bvar {z : V} (hz : z < n) : L.termShift n (^#z) = ^#z :=
-  Language.IsSemiterm.termShift_eq_of (by simp [hz]) (Shift.bvar hz)
-
-@[simp] lemma termShift_fvar (x : V) : L.termShift n (^&x) = ^&(x + 1) :=
-  Language.IsSemiterm.termShift_eq_of (by simp) (Shift.fvar x)
-
-lemma termShift_func {k f v v' : V} (hfk : L.Func k f)
-    (hv : L.TermSeq k n v)
-    (hv' : L.TermSeq k n v')
-    (H : ∀ i u u', ⟪i, u⟫ ∈ v → ⟪i, u'⟫ ∈ v' → L.termShift n u = u') : L.termShift n (^func k f v) = ^func k f v' :=
-  Language.IsSemiterm.termShift_eq_of (IsSemiterm.func hfk hv)
-    (Shift.func hfk hv hv' (fun i u u' hi hi' ↦ by
-      rcases H i u u' hi hi'
-      exact Language.IsSemiterm.termShift_spec (hv.prop i u hi)))
-
-section
-
-variable (L)
-
-private lemma termShift_graph (u n t : V) :
-    u = L.termShift n t ↔
-    (L.IsSemiterm n t → ∃ p ≤ (t + u + 1)^2, p = ⟪t, u⟫ ∧ Shift L n p) ∧ (¬L.IsSemiterm n t → u = 0) :=
-  Iff.trans (Classical.choose!_eq_iff (Shift.rng_exists_unique_total L n t)) ⟨by
-    rintro ⟨hp, hn⟩
-    exact ⟨fun h ↦ ⟨⟪t, u⟫, by simp, rfl, hp h⟩, hn⟩, by
-    rintro ⟨hp, hn⟩
-    exact ⟨fun h ↦ by rcases hp h with ⟨_, _, rfl, h⟩; exact h, hn⟩⟩
-
-def _root_.LO.FirstOrder.Arith.LDef.termShiftDef (pL : LDef) : 𝚺₁-Semisentence 3 := .mkSigma
-  “u n t | (!pL.isSemitermDef.pi n t → ∃ p <⁺ (t + u + 1)², !pairDef p t u ∧ !(shiftDef pL).sigma n p) ∧ (¬!pL.isSemitermDef.sigma n t → u = 0)” (by simp)
-
-lemma termShift_defined : 𝚺₁-Function₂ L.termShift via pL.termShiftDef := by
-  intro v
-  simp [LDef.termShiftDef, termShift_graph, HSemiformula.val_sigma, eval_termSeq L,
-    eval_isSemitermDef L, (termSeq_defined L).proper.iff', (isSemiterm_defined L).proper.iff', eval_shiftDef L, -and_imp, -not_and]
-
-@[simp] lemma termShift_defined_iff (v : Fin 3 → V) :
-    Semiformula.Evalbm (L := ℒₒᵣ) V v pL.termShiftDef ↔ v 0 = L.termShift (v 1) (v 2) := (termShift_defined L).df.iff v
-
-instance termShift_definable : 𝚺₁-Function₂ L.termShift :=
-  Defined.to_definable _ (termShift_defined L)
-
-end
-
-end termShift
--/
 
 end LO.Arith
 
