Arithmetization/ISigmaOne/Metamath/Formula/Functions.lean
@@ -1,0 +1,111 @@
+import Arithmetization.ISigmaOne.Metamath.Formula.Basic
+import Arithmetization.ISigmaOne.Metamath.Term.Functions
+
+noncomputable section
+
+namespace LO.Arith
+
+open FirstOrder FirstOrder.Arith
+
+variable {V : Type*} [Zero V] [One V] [Add V] [Mul V] [LT V] [V ⊧ₘ* 𝐈𝚺₁]
+
+variable {L : Arith.Language V} {pL : LDef} [Arith.Language.Defined L pL]
+
+namespace Negation
+
+def blueprint (pL : LDef) : Language.UformulaRec.Blueprint pL 0 where
+  rel := .mkSigma “y n k R v | !qqNRelDef y n k R v” (by simp)
+  nrel := .mkSigma “y n k R v | !qqRelDef y n k R v” (by simp)
+  verum := .mkSigma “y n | !qqFalsumDef y n” (by simp)
+  falsum := .mkSigma “y n | !qqVerumDef y n” (by simp)
+  and := .mkSigma “y n p₁ p₂ y₁ y₂ | !qqOrDef y n y₁ y₂” (by simp)
+  or := .mkSigma “y n p₁ p₂ y₁ y₂ | !qqAndDef y n y₁ y₂” (by simp)
+  all := .mkSigma “y n p₁ y₁ | !qqExDef y n y₁” (by simp)
+  ex := .mkSigma “y n p₁ y₁ | !qqAllDef y n y₁” (by simp)
+
+variable (L)
+
+def construction : Language.UformulaRec.Construction V L (blueprint pL) where
+  rel {_} := fun n k R v ↦ ^nrel n k R v
+  nrel {_} := fun n k R v ↦ ^rel n k R v
+  verum {_} := fun n ↦ ^⊥[n]
+  falsum {_} := fun n ↦ ^⊤[n]
+  and {_} := fun n _ _ y₁ y₂ ↦ y₁ ^⋎[n] y₂
+  or {_} := fun n _ _ y₁ y₂ ↦ y₁ ^⋏[n] y₂
+  all {_} := fun n _ y₁ ↦ ^∃[n] y₁
+  ex {_} := fun n _ y₁ ↦ ^∀[n] y₁
+  rel_defined := by intro v; simp [blueprint]; rfl
+  nrel_defined := by intro v; simp [blueprint]; rfl
+  verum_defined := by intro v; simp [blueprint]
+  falsum_defined := by intro v; simp [blueprint]
+  and_defined := by intro v; simp [blueprint]; rfl
+  or_defined := by intro v; simp [blueprint]; rfl
+  all_defined := by intro v; simp [blueprint]; rfl
+  ex_defined := by intro v; simp [blueprint]; rfl
+
+end Negation
+
+section negation
+
+open Negation
+
+variable (L)
+
+def Language.neg (p : V) : V := (construction L).result ![] p
+
+variable {L}
+
+@[simp] lemma neg_rel {n k R v} (hR : L.Rel k R) (hv : L.TermSeq k n v) :
+    L.neg (^rel n k R v) = ^nrel n k R v := by simp [Language.neg, hR, hv, construction]
+
+@[simp] lemma neg_nrel {n k R v} (hR : L.Rel k R) (hv : L.TermSeq k n v) :
+    L.neg (^nrel n k R v) = ^rel n k R v := by simp [Language.neg, hR, hv, construction]
+
+@[simp] lemma neg_verum (n) :
+    L.neg ^⊤[n] = ^⊥[n] := by simp [Language.neg, construction]
+
+@[simp] lemma neg_falsum (n) :
+    L.neg ^⊥[n] = ^⊤[n] := by simp [Language.neg, construction]
+
+@[simp] lemma neg_and {n p q} (hp : L.Semiformula n p) (hq : L.Semiformula n q) :
+    L.neg (p ^⋏[n] q) = L.neg p ^⋎[n] L.neg q := by simp [Language.neg, hp, hq, construction]
+
+@[simp] lemma neg_or {n p q} (hp : L.Semiformula n p) (hq : L.Semiformula n q) :
+    L.neg (p ^⋎[n] q) = L.neg p ^⋏[n] L.neg q := by simp [Language.neg, hp, hq, construction]
+
+@[simp] lemma neg_all {n p} (hp : L.Semiformula (n + 1) p) :
+    L.neg (^∀[n] p) = ^∃[n] (L.neg p) := by simp [Language.neg, hp, construction]
+
+@[simp] lemma neg_ex {n p} (hp : L.Semiformula (n + 1) p) :
+    L.neg (^∃[n] p) = ^∀[n] (L.neg p) := by simp [Language.neg, hp, construction]
+
+section
+
+def _root_.LO.FirstOrder.Arith.LDef.negDef (pL : LDef) : 𝚺₁-Semisentence 2 := (blueprint pL).result
+
+variable (L)
+
+lemma neg_defined : 𝚺₁-Function₁ L.neg via pL.negDef := (construction L).result_defined
+
+@[simp] lemma neg_defined_iff (v : Fin 2 → V) :
+    Semiformula.Evalbm (L := ℒₒᵣ) V v pL.negDef ↔ v 0 = L.neg (v 1) := (neg_defined L).df.iff v
+
+instance neg_definable : 𝚺₁-Function₁ L.neg :=
+  Defined.to_definable _ (neg_defined L)
+
+@[simp, definability] instance neg_definable' (Γ) : (Γ, m + 1)-Function₁ L.neg :=
+  .of_sigmaOne (neg_definable L) _ _
+
+end
+
+end negation
+
+section substs
+
+
+
+end substs
+
+end LO.Arith
+
+end
